backends/lean/Aeneas/Tactic/Step/UnfoldPF.lean
@@ -1,0 +1,310 @@
+import Lean
+import Aeneas.Tactic.Solver.ScalarTac
+import Aeneas.Tactic.Step.Init
+import Aeneas.Tactic.Step.GrindState
+import Aeneas.Std
+import Aeneas.Tactic.Simp.SimpLemmas
+import AeneasMeta.Async
+import Aeneas.Tactic.Solver.Grind.Init
+import Aeneas.Tactic.Step.InferPost
+import Aeneas.Tactic.Step
+
+-- tactic for unfolding partial_fixpoint definitions with fixpoint_induct
+-- normally you would use the normal unfold tactic, but that requires the proof to be terminating
+
+namespace Aeneas
+
+namespace UnfoldPF
+
+open Lean Elab Term Meta Tactic
+open Utils
+open Lean.Order
+open Std Result
+
+
+  theorem curry_admissible (a1 a2 a3) (P : (a1 → a2 → a3) → Prop) [CCPO a3]
+    (h : Order.admissible fun (f : (a1 × a2) → a3) => P (fun x y => f (x, y)))
+    : Order.admissible fun (f : a1 → a2 → a3) => P f := by
+    intros c hchain hc
+    simp only at hc
+    unfold admissible at h
+    simp only at h
+    have h := h (fun f => c (fun x y => f (x, y))) (
+      by
+        unfold chain
+        unfold chain at hchain
+        intros s1 s2 cs1 cs2
+        have thing := hchain (fun x y => s1 (x, y)) (fun x y => s2 (x, y)) cs1 cs2
+        unfold PartialOrder.rel
+        unfold instCCPOPi
+        simp only
+        unfold instOrderPi
+        simp only
+        cases thing with
+        | inl thing =>
+            apply Or.inl
+            intros
+            apply thing
+        | inr thing =>
+          apply Or.inr
+          intros
+          apply thing
+    ) ( by
+      intros f
+      apply hc
+    )
+    simp at h
+    --
+    rw [← Order.fun_csup_eq]
+    unfold fun_csup
+    simp only
+    --
+    simp only [← Order.fun_csup_eq]
+    unfold fun_csup
+    simp only
+    --
+    simp only [← Order.fun_csup_eq] at h
+    unfold fun_csup at h
+    simp only at h
+    --
+    have lemma1 (x : a1) (y : a2)
+      : (fun z => ∃ (f : a1 × a2 → a3), (c fun x y => f (x, y)) ∧ f (x, y) = z)
+        = (fun z => ∃ f, (∃ f_1, c f_1 ∧ f_1 x = f) ∧ f y = z) := by
+      simp
+      funext z
+      simp only [eq_iff_iff]
+      apply Iff.intro
+      · intros h
+        rcases h with ⟨f, a, b⟩
+        exists (fun x y => f (x, y))
+      ·
+        intros h
+        rcases h with ⟨f, a, b⟩
+        exists (fun p => f p.fst p.snd)
+        --
+      --
+    simp [lemma1] at h
+    simp only [↓existsAndEq, and_true] at *
+    apply h
+
+  theorem WP_func_admissible (α β) (arg) (post)
+    : Order.admissible fun (f : α → Result β) => WP.dspec (f arg) post := by
+    apply Lean.Order.admissible_apply (fun _ fx => WP.dspec fx _)
+    apply Lean.Order.admissible_flatOrder
+    simp only [WP.dspec]
+
+  macro "prove_admissible" : tactic =>
+    `(tactic| (
+        (repeat' apply curry_admissible)
+        (repeat' (apply Lean.Order.admissible_pi ; intro))
+        (apply WP_func_admissible)
+    )
+    )
+
+  elab "unfold_div_old" : tactic => do
+    let mut goal ← getMainGoal
+    let ty ← goal.getType
+
+    let (thHead, thArgs) := ty.consumeMData.withApp (fun f args => (f, args))
+    -- TODO: here is where it should be able to lift from spec to dspec
+    if !thHead.isConst || thHead.constName! != ``Std.WP.dspec then
+      throwError "Not dspec statement"
+    -- let .app WP.dspec a b := ty
+    let (func, funcargs) := thArgs[1]!.consumeMData.withApp (fun f args => (f, args))
+    if !func.isConst then
+      throwError "Can only unfold (dspec (func... ) post) when func is a constant"
+
+    let post := thArgs[2]!
+    -- the goal is now split into (dspec (func ..funcargs) post)
+
+    -- let mut vars : Array FVarId := #[]
+
+    -- should we automatically revert variables? could this ever cause a problem?
+    -- -- first, we need to revert free variables that are arguments to the function
+    -- for arg in funcargs do
+    --   -- TODO: maybe its not always a free var, what cases need to be handled here?
+    --   let var := arg.fvarId!
+    --   vars := vars.push var
+    --   (_, goal) ← goal.revert #[var]
+
+
+    -- do some wierd hacky nonsense to get `func.fixpoint_induct`
+    let namee := func.constName!.mkStr "fixpoint_induct"
+    let fi_stx : Syntax ← `(term | $(mkIdent namee))
+    let fixpoint_induct ← Term.elabTerm fi_stx none
+    trace[UnfoldPF] "type of fixpoint_induct is {← inferType fixpoint_induct}"
+
+    -- apply fixpoint_induct
+    let fi_app := mkAppN fixpoint_induct #[
+      .lam `func (← inferType func)
+      (mkAppN (.bvar 0) #[])
+      .default
+    ]
+
+    replaceMainGoal [goal]
+    pure ()
+
+  -- this new version doesn't try to revert the variables, and is more general.
+  -- but it requires that you give it the name of the thing to induct over
+  elab "fixpoint_induction" func:ident : tactic => do
+    let mut goal ← getMainGoal
+    let ty ← goal.getType
+
+    let func_expr ← Term.elabTerm func none
+
+    -- do some wierd hacky nonsense to get `func.fixpoint_induct`
+    let namee := func.getId.mkStr "fixpoint_induct"
+    let fi_stx : Syntax ← `(term | $(mkIdent namee))
+    let fixpoint_induct ← Term.elabTerm fi_stx none
+    trace[UnfoldPF] "type of fixpoint_induct is {← inferType fixpoint_induct}"
+    -- apply fixpoint_induct
+
+    -- make a type family that abstracts over instances of func in the goal type
+    let abs_goal_ty := ty.abstract #[func_expr]
+
+    let fi_app := mkAppN fixpoint_induct #[.lam `func (← inferType func_expr)
+      (abs_goal_ty.instantiate1 (.bvar 0)) .default
+    ]
+
+    let [g1, g2] ← goal.apply fi_app
+      | throwError "bla"
+
+    setGoals [g1]
+    evalTactic (← `(tactic|prove_admissible))
+
+    replaceMainGoal [g2]
+    pure ()
+
+  set_option trace.UnfoldPF true
+  -- #check simple_diverge.fixpoint_induct
+
+  theorem test_div_2 (x : Std.I32) : Std.WP.dspec (simple_diverge x) (fun res => res = 10#i32)
+    := by
+    unfold_div
+    --
+    sorry
+
+namespace Test
+
+  open Std Result Aeneas.UnfoldPF
+  def simple_diverge (x : Std.I32) : Result Std.I32 := do
+    if x = 0#i32
+    then ok 10#i32
+    else
+      let i1 ← 1#i32 + 1#i32
+      simple_diverge i1
+  partial_fixpoint
+
+  theorem test_div2 (x : Std.I32) : Std.WP.dspec (simple_diverge x) (fun res => res = 10#i32)
+    := by
+      unfold simple_diverge
+      --
+      sorry
+
+  -- TODO: if i use unfold then sorry, print proof term, i can see how it proves admissibility
+  #check simple_diverge.fixpoint_induct
+  @[step]
+  theorem test_div (x : Std.I32) : Std.WP.dspec (simple_diverge x) (fun res => res = 10#i32)
+    := by
+      --
+      revert x
+      apply simple_diverge.fixpoint_induct
+        (motive := fun simple_diverge => ∀ x, WP.dspec (simple_diverge x) (fun res => res = 10#i32))
+      · apply Lean.Order.admissible_pi
+        intros y
+        apply Lean.Order.admissible_apply (fun _ fx => WP.dspec fx _)
+        apply Lean.Order.admissible_flatOrder
+        simp only [WP.dspec]
+      · intros
+        simp only
+        split
+        . simp [*]
+        . step
+          step
+          simp [*]
+
+  theorem test_div_no_revert (x : Std.I32) : Std.WP.dspec (simple_diverge x) (fun res => res = 10#i32)
+    := by
+      --
+      apply simple_diverge.fixpoint_induct
+        (motive := fun simple_diverge => ∀ x, WP.dspec (simple_diverge x) (fun res => res = 10#i32))
+      · apply Lean.Order.admissible_pi
+        intros y
+        apply Lean.Order.admissible_apply (fun _ fx => WP.dspec fx _)
+        apply Lean.Order.admissible_flatOrder
+        simp only [WP.dspec]
+        --
+      · intros
+        simp only
+        split
+        . simp [*]
+        . step
+          step
+          simp [*]
+
+  theorem test_div_no_revert_no_all (x : Std.I32) : Std.WP.dspec (simple_diverge x) (fun res => res = 10#i32)
+    := by
+      --
+      apply simple_diverge.fixpoint_induct
+        (motive := fun simple_diverge => WP.dspec (simple_diverge x) (fun res => res = 10#i32))
+      · apply Lean.Order.admissible_apply (fun _ fx => WP.dspec fx _)
+        apply Lean.Order.admissible_flatOrder
+        simp only [WP.dspec]
+      · intros
+        simp only
+        split
+        . simp [*]
+        . step
+          step
+          simp [*]
+  def simple_diverge_2 (x y : Std.I32) : Result Std.I32 := do
+    if x = y#i32
+    then ok 10#i32
+    else
+      let i1 ← 1#i32 + 1#i32
+      let i2 ← 1#i32 + 1#i32
+      simple_diverge_2 i1 i2
+  partial_fixpoint
+
+  def admissible_apply_simpler {α : Sort u}{β : Sort v} [CCPO β] (P : β → Prop) (x : α)
+    (hadm : admissible P) : admissible (fun (f : α → β) => P (f x)) := by
+    apply admissible_apply (fun _ => P) x
+    assumption
+
+  theorem test_add_2 (a1 a2 β) (post)
+    : Order.admissible fun (f : a1 → a2 → Result β) => ∀ (x : a1) (y : a2), WP.dspec (f x y) post := by
+    apply Lean.Order.admissible_pi
+    intros y1
+    apply Lean.Order.admissible_pi
+    intros y2
+    --
+    apply admissible_apply_simpler (β := a2 → Result β) (fun fx => WP.dspec (fx y2) post) y1
+    -- apply Lean.Order.admissible_apply (β := fun _ => a2 → Result β)
+      -- (fun x fx => WP.dspec (fx y2) post) y1
+    apply Lean.Order.admissible_apply (fun _ fx => WP.dspec fx _)
+    apply Lean.Order.admissible_flatOrder
+    simp only [WP.dspec]
+
+  theorem test_div_2 (x y : Std.I32) : Std.WP.dspec (simple_diverge_2 x y) (fun res => res = 10#i32)
+    := by
+      --
+      revert x y
+      apply simple_diverge_2.fixpoint_induct
+        (motive := fun simple_diverge_2 => ∀ x y, WP.dspec (simple_diverge_2 x y) (fun res => res = 10#i32))
+      ·
+        -- apply test_add_2
+        prove_admissible
+        --
+      · intros
+        simp only
+        split
+        . simp [*]
+        . step
+          step
+          simp [*]
+          --
+end Test
+
+
+end UnfoldPF
+end Aeneas
